Checkpoint in allocate_bytes proof.

src/coq/Handlers/MemoryInterpreters.v
@@ -55,18 +55,20 @@ Module Type MemorySpecInterpreter (LP : LLVMParams) (MP : MemoryParams LP) (MMSP
     Notation Effout := (E +' F).
 
     Definition MemStateT M := stateT MemState M.
-    Definition MemStateFreshT M := stateT store_id (MemStateT M).
+    Definition MemStateFreshT M := stateT store_id (stateT Provenance (MemStateT M)).
 
     Definition MemStateFreshT_from_MemStateT {M X} `{Monad M} (mst : MemStateT M X) : MemStateFreshT M X :=
-      fun sid => x <- mst;; ret (sid, x).
+      fun sid pr => x <- mst;; ret (pr, (sid, x)).
 
     (** MemMonad Instances *)
     #[global] Instance MemStateFreshT_Provenance M `{Monad M} : MonadProvenance Provenance (MemStateFreshT M).
     Proof.
       split.
-      unfold MemStateFreshT.
-      apply (lift (ms <- get;;
-                   ret (get_fresh_provenance ms))).
+      exact (lift
+               (pr <- get;;
+                let pr' := next_provenance pr in
+                put pr';;
+                ret pr')).
     Defined.
 
     #[global] Instance MemStateFreshT_MonadStoreId M `{Monad M} : MonadStoreId (MemStateFreshT M).
@@ -82,8 +84,8 @@ Module Type MemorySpecInterpreter (LP : LLVMParams) (MP : MemoryParams LP) (MMSP
     #[global] Instance MemStateFreshT_MonadMemState M `{Monad M} : MonadMemState MemState (MemStateFreshT M).
     Proof.
       split.
-      - apply (lift get).
-      - intros ms; apply (lift (put ms)).
+      - apply (lift (lift get)).
+      - intros ms; apply (lift (lift (put ms))).
     Defined.
 
     #[global] Instance MemState_StoreIdFreshness : StoreIdFreshness MemState.
@@ -92,11 +94,13 @@ Module Type MemorySpecInterpreter (LP : LLVMParams) (MP : MemoryParams LP) (MMSP
       apply used_store_id_prop.
     Defined.
 
-    #[global] Instance MemState_ProvenanceFreshness : ProvenanceFreshness Provenance MemState.
+    Definition MemStateFreshT_State := (store_id * Provenance)%type.
+
+    #[global] Instance MemState_ProvenanceFreshness : ProvenanceFreshness Provenance MemStateFreshT_State.
     Proof.
       split.
-      - (* Is a provenance used in a memstate *)
-        apply MMSP.used_provenance_prop.
+      - intros [sid pr] pr'.
+        exact (provenance_lt pr (next_provenance pr')).
     Defined.
 
     #[global] Instance MemStateFreshT_MonadT {M} `{Monad M} : MonadT (MemStateFreshT M) M.
@@ -105,26 +109,26 @@ Module Type MemorySpecInterpreter (LP : LLVMParams) (MP : MemoryParams LP) (MMSP
       unfold MemStateT.
       split.
       - intros t X.
-        intros sid ms.
-        apply (res <- X;; ret (ms, (sid, res))).
+        intros sid pr ms.
+        apply (res <- X;; ret (ms, (pr, (sid, res)))).
     Defined.
-
-    Definition MemStateFreshT_State := store_id.
 
     (* M may be PropT or itree... *)
     Definition MemStateFreshT_run {A} {Eff} `{FailureE -< Eff} `{OOME -< Eff} `{UBE -< Eff} (ma : MemStateFreshT (itree Eff) A) (ms : MemState) (st : MemStateFreshT_State) : itree Eff (MemStateFreshT_State * (MemState * A)).
     Proof.
       unfold MemStateFreshT in *.
-      specialize (ma st ms).
+      destruct st as [sid pr].
+      specialize (ma sid pr ms).
       unfold MemStateFreshT_State.
       eapply fmap; [ |eauto].
-      intros [ms' [s' x]].
-      apply (s', (ms', x)).
+      intros [ms' [pr' [s' x]]].
+      apply ((s', pr'), (ms', x)).
     Defined.
 
     Definition MemStateFreshT_valid_state (ms : MemState) (st : MemStateFreshT_State) : Prop
-      := let sid := st in
-         (forall sid', used_store_id ms sid' -> (sid' < sid)%N).
+      := let '(sid, pr) := st in
+         (forall sid', used_store_id ms sid' -> (sid' < sid)%N) /\
+           (forall pr', used_provenance st pr' -> (provenance_lt pr' pr)%N).
 
     #[global] Instance MemStateFreshT_MemMonad {Eff} `{FAIL: FailureE -< Eff} `{OOM: OOME -< Eff} `{UB: UBE -< Eff}
       : MemMonad MemState MemStateFreshT_State Provenance (MemStateFreshT (itree Eff)) (itree Eff).
@@ -135,7 +139,7 @@ Module Type MemorySpecInterpreter (LP : LLVMParams) (MP : MemoryParams LP) (MMSP
 
       (* TODO: didn't need valid for ret / bind laws... *)
       - (* run bind *)
-        intros A B ma k ms st VALID.
+        intros A B ma k ms [sid pr] VALID.
         unfold MemStateFreshT_run.
         cbn.
         rewrite map_bind.
@@ -143,16 +147,16 @@ Module Type MemorySpecInterpreter (LP : LLVMParams) (MP : MemoryParams LP) (MMSP
         eapply eutt_clo_bind.
         reflexivity.
         intros u1 u2 H2; subst.
-        destruct u2 as [ms' [sid' x]].
+        destruct u2 as [ms' [pr' [sid' x]]].
         cbn.
         reflexivity.
       - (* run ret *)
-        intros A x ms st VALID.
+        intros A x ms [sid pr] VALID.
         cbn.
         rewrite map_ret.
         reflexivity.
       - (* get_mem_state *)
-        intros ms sid.
+        intros ms [sid pr].
         cbn.
         rewrite map_bind.
         repeat rewrite bind_ret_l.
@@ -160,7 +164,7 @@ Module Type MemorySpecInterpreter (LP : LLVMParams) (MP : MemoryParams LP) (MMSP
         cbn.
         reflexivity.
       - (* put_mem_state *)
-        intros ms ms' sid.
+        intros ms ms' [sid pr].
         cbn.
         rewrite map_bind.
         repeat rewrite bind_ret_l.
@@ -168,7 +172,7 @@ Module Type MemorySpecInterpreter (LP : LLVMParams) (MP : MemoryParams LP) (MMSP
         cbn.
         reflexivity.
       - (* fresh_sid *)
-        intros ms sid VALID.
+        intros ms [sid pr] VALID.
         do 2 eexists.
         cbn.
         rewrite map_bind.
@@ -180,30 +184,52 @@ Module Type MemorySpecInterpreter (LP : LLVMParams) (MP : MemoryParams LP) (MMSP
         split; [reflexivity|].
 
         cbn in VALID.
+        destruct VALID as [VALID_SID VALID_PR].
         split.
         + red.
-          intros sid' USED.
-          apply VALID in USED.
-          lia.
+          split.
+          * intros sid' USED.
+            apply VALID_SID in USED.
+            lia.
+          * intros pr' USED.
+            apply VALID_PR in USED.
+            auto.
         + intros USED.
-          apply VALID in USED.
+          apply VALID_SID in USED.
           lia.
-      - (* fresh_provenance *)
-        intros ms sid VALID.
-        do 2 eexists.
-        cbn.
-        rewrite map_bind.
-        repeat rewrite bind_ret_l.
-        rewrite map_ret.
-        cbn.
-        split; [reflexivity|].
+      (* - (* fresh_provenance *) *)
+      (*   intros ms [sid pr] [VALID_SID VALID_PR]. *)
+      (*   do 2 eexists. *)
+      (*   cbn. *)
+      (*   rewrite map_bind. *)
+      (*   repeat setoid_rewrite bind_ret_l. *)
+      (*   cbn. *)
 
-        cbn in VALID.
-        split.
-        + auto.
-        + apply get_fresh_provenance_fresh.
+      (*   split; [|split]. *)
+      (*   + reflexivity. *)
+      (*   + split. *)
+      (*     * intros sid' USED. *)
+      (*       apply VALID_SID in USED. *)
+      (*       auto. *)
+      (*     * intros pr' USED. *)
+      (*       assert (used_provenance (sid, pr) pr') as USED'. *)
+      (*       { cbn in USED. cbn. *)
+      (*         eapply provenance_lt_trans. *)
+      (*         eapply provenance_lt_next_provenance. *)
+      (*         eauto. *)
+      (*       } *)
+      (*       apply VALID_PR in USED'. *)
+      (*       eapply provenance_lt_trans; eauto. *)
+      (*       eapply provenance_lt_next_provenance. *)
+      (*   + split. *)
+      (*     * intros CONTRA. *)
+      (*       apply VALID_PR in CONTRA. *)
+      (*       pose proof provenance_lt_next_provenance pr as CONTRA2. *)
+      (*       pose proof provenance_lt_antisym _ _ CONTRA CONTRA2 as EQ. *)
+      (*       eapply next_provenance_neq; eauto. *)
+      (*     * eapply provenance_lt_next_provenance. *)
       - (* raise_oom *)
-        intros A ms oom_msg sid.
+        intros A ms oom_msg [sid pr].
         cbn.
         rewrite map_bind.
         setoid_rewrite Raise.raiseOOM_bind_itree.
@@ -213,13 +239,13 @@ Module Type MemorySpecInterpreter (LP : LLVMParams) (MP : MemoryParams LP) (MMSP
         intros EQ.
         pinversion EQ.
       - (* raise_ub *)
-        intros A ms oom_msg sid.
+        intros A ms oom_msg [sid pr].
         cbn.
         rewrite map_bind.
         setoid_rewrite Raise.raiseUB_bind_itree.
         reflexivity.
       - (* raise_error *)
-        intros A ms oom_msg sid.
+        intros A ms oom_msg [sid pr].
         cbn.
         rewrite map_bind.
         setoid_rewrite Raise.raise_bind_itree.
@@ -237,10 +263,10 @@ Module Type MemorySpecInterpreter (LP : LLVMParams) (MP : MemoryParams LP) (MMSP
       fun R e m => fun t => t ≈ r <- trigger e;; ret (m, r).
 
     Definition E_trigger : forall R, E R -> (MemStateFreshT (PropT Effout) R) :=
-      fun R e sid m => fun t => t ≈ r <- trigger e;; ret (m, (sid, r)).
+      fun R e sid pr m => fun t => t ≈ r <- trigger e;; ret (m, (pr, (sid, r))).
 
     Definition F_trigger : forall R, F R -> (MemStateFreshT (PropT Effout) R) :=
-      fun R e sid m => fun t => t ≈ r <- trigger e;; ret (m, (sid, r)).
+      fun R e sid pr m => fun t => t ≈ r <- trigger e;; ret (m, (pr, (sid, r))).
 
     (* TODO: get rid of this silly hack. *)
     Definition my_handle_memory_prop' :
@@ -313,8 +339,9 @@ Module Type MemorySpecInterpreter (LP : LLVMParams) (MP : MemoryParams LP) (MMSP
        type signature as interp_memory... *)
     Definition interp_memory_prop {R} (RR : R -> R -> Prop) :
       itree Effin R -> MemStateFreshT (PropT Effout) R :=
-      fun (t : itree Effin R) (sid : store_id) (ms : MemState) (t' : itree Effout (MemState * (store_id * R))) =>
-        interp_prop (fun T (e : Effin T) (t : itree Effout T) => exists (sid' : store_id) (ms' : MemState), @interp_memory_prop_h T e sid ms (fmap (fun (x : T) => (ms', (sid', x))) t)) (@memory_k_spec) R RR t ((fmap (fun '(_, (_, x)) => x) t') : itree Effout R).
+      fun (t : itree Effin R) (sid : store_id) (pr : Provenance) (ms : MemState) (t' : itree Effout (MemState * (Provenance * (store_id * R)))) =>
+        interp_prop (fun T (e : Effin T) (t : itree Effout T) => exists (sid' : store_id) (pr' : Provenance) (ms' : MemState),
+                         @interp_memory_prop_h T e sid pr ms (fmap (fun (x : T) => (ms', (pr', (sid', x)))) t)) (@memory_k_spec) R RR t ((fmap (fun '(_, (_, (_, x))) => x) t') : itree Effout R).
   End Interpreters.
 End MemorySpecInterpreter.
 
@@ -343,9 +370,11 @@ Module Type MemoryExecInterpreter (LP : LLVMParams) (MP : MemoryParams LP) (MMEP
     #[global] Instance MemStateFreshT_Provenance M `{Monad M} : MonadProvenance Provenance (MemStateFreshT M).
     Proof.
       split.
-      unfold MemStateFreshT.
-      apply (lift (ms <- get;;
-                   ret (get_fresh_provenance ms))).
+      exact (lift
+               (pr <- get;;
+                let pr' := next_provenance pr in
+                put pr';;
+                ret pr')).
     Defined.
 
     #[global] Instance MemStateFreshT_MonadStoreId M `{Monad M} : MonadStoreId (MemStateFreshT M).
@@ -361,8 +390,8 @@ Module Type MemoryExecInterpreter (LP : LLVMParams) (MP : MemoryParams LP) (MMEP
     #[global] Instance MemStateFreshT_MonadMemState M `{Monad M} : MonadMemState MemState (MemStateFreshT M).
     Proof.
       split.
-      - apply (lift get).
-      - intros ms; apply (lift (put ms)).
+      - apply (lift (lift get)).
+      - intros ms; apply (lift (lift (put ms))).
     Defined.
 
     #[global] Instance MemState_StoreIdFreshness : StoreIdFreshness MemState.
@@ -371,11 +400,13 @@ Module Type MemoryExecInterpreter (LP : LLVMParams) (MP : MemoryParams LP) (MMEP
       apply used_store_id_prop.
     Defined.
 
-    #[global] Instance MemState_ProvenanceFreshness : ProvenanceFreshness Provenance MemState.
+    Definition MemStateFreshT_State := (store_id * Provenance)%type.
+
+    #[global] Instance MemState_ProvenanceFreshness : ProvenanceFreshness Provenance MemStateFreshT_State.
     Proof.
       split.
-      - (* Is a provenance used in a memstate *)
-        apply MMSP.used_provenance_prop.
+      - intros [sid pr] pr'.
+        exact (provenance_lt pr (next_provenance pr')).
     Defined.
 
     #[global] Instance MemStateFreshT_MonadT {M} `{Monad M} : MonadT (MemStateFreshT M) M.
@@ -384,26 +415,26 @@ Module Type MemoryExecInterpreter (LP : LLVMParams) (MP : MemoryParams LP) (MMEP
       unfold MemStateT.
       split.
       - intros t X.
-        intros sid ms.
-        apply (res <- X;; ret (ms, (sid, res))).
+        intros sid pr ms.
+        apply (res <- X;; ret (ms, (pr, (sid, res)))).
     Defined.
-
-    Definition MemStateFreshT_State := store_id.
 
     (* M may be PropT or itree... *)
     Definition MemStateFreshT_run {A} {Eff} `{FailureE -< Eff} `{OOME -< Eff} `{UBE -< Eff} (ma : MemStateFreshT (itree Eff) A) (ms : MemState) (st : MemStateFreshT_State) : itree Eff (MemStateFreshT_State * (MemState * A)).
     Proof.
       unfold MemStateFreshT in *.
-      specialize (ma st ms).
+      destruct st as [sid pr].
+      specialize (ma sid pr ms).
       unfold MemStateFreshT_State.
       eapply fmap; [ |eauto].
-      intros [ms' [s' x]].
-      apply (s', (ms', x)).
+      intros [ms' [pr' [s' x]]].
+      apply ((s', pr'), (ms', x)).
     Defined.
 
     Definition MemStateFreshT_valid_state (ms : MemState) (st : MemStateFreshT_State) : Prop
-      := let sid := st in
-         (forall sid', used_store_id ms sid' -> (sid' < sid)%N).
+      := let '(sid, pr) := st in
+         (forall sid', used_store_id ms sid' -> (sid' < sid)%N) /\
+           (forall pr', used_provenance st pr' -> (provenance_lt pr' pr)%N).
 
     #[global] Instance MemStateFreshT_MemMonad {Eff} `{FAIL: FailureE -< Eff} `{OOM: OOME -< Eff} `{UB: UBE -< Eff}
       : MemMonad MemState MemStateFreshT_State Provenance (MemStateFreshT (itree Eff)) (itree Eff).
@@ -414,7 +445,7 @@ Module Type MemoryExecInterpreter (LP : LLVMParams) (MP : MemoryParams LP) (MMEP
 
       (* TODO: didn't need valid for ret / bind laws... *)
       - (* run bind *)
-        intros A B ma k ms st VALID.
+        intros A B ma k ms [sid pr] VALID.
         unfold MemStateFreshT_run.
         cbn.
         rewrite map_bind.
@@ -422,16 +453,16 @@ Module Type MemoryExecInterpreter (LP : LLVMParams) (MP : MemoryParams LP) (MMEP
         eapply eutt_clo_bind.
         reflexivity.
         intros u1 u2 H2; subst.
-        destruct u2 as [ms' [sid' x]].
+        destruct u2 as [ms' [pr' [sid' x]]].
         cbn.
         reflexivity.
       - (* run ret *)
-        intros A x ms st VALID.
+        intros A x ms [sid pr] VALID.
         cbn.
         rewrite map_ret.
         reflexivity.
       - (* get_mem_state *)
-        intros ms sid.
+        intros ms [sid pr].
         cbn.
         rewrite map_bind.
         repeat rewrite bind_ret_l.
@@ -439,7 +470,7 @@ Module Type MemoryExecInterpreter (LP : LLVMParams) (MP : MemoryParams LP) (MMEP
         cbn.
         reflexivity.
       - (* put_mem_state *)
-        intros ms ms' sid.
+        intros ms ms' [sid pr].
         cbn.
         rewrite map_bind.
         repeat rewrite bind_ret_l.
@@ -447,7 +478,7 @@ Module Type MemoryExecInterpreter (LP : LLVMParams) (MP : MemoryParams LP) (MMEP
         cbn.
         reflexivity.
       - (* fresh_sid *)
-        intros ms sid VALID.
+        intros ms [sid pr] VALID.
         do 2 eexists.
         cbn.
         rewrite map_bind.
@@ -459,30 +490,52 @@ Module Type MemoryExecInterpreter (LP : LLVMParams) (MP : MemoryParams LP) (MMEP
         split; [reflexivity|].
 
         cbn in VALID.
+        destruct VALID as [VALID_SID VALID_PR].
         split.
         + red.
-          intros sid' USED.
-          apply VALID in USED.
-          lia.
+          split.
+          * intros sid' USED.
+            apply VALID_SID in USED.
+            lia.
+          * intros pr' USED.
+            apply VALID_PR in USED.
+            auto.
         + intros USED.
-          apply VALID in USED.
+          apply VALID_SID in USED.
           lia.
-      - (* fresh_provenance *)
-        intros ms sid VALID.
-        do 2 eexists.
-        cbn.
-        rewrite map_bind.
-        repeat rewrite bind_ret_l.
-        rewrite map_ret.
-        cbn.
-        split; [reflexivity|].
+      (* - (* fresh_provenance *) *)
+      (*   intros ms [sid pr] [VALID_SID VALID_PR]. *)
+      (*   do 2 eexists. *)
+      (*   cbn. *)
+      (*   rewrite map_bind. *)
+      (*   repeat setoid_rewrite bind_ret_l. *)
+      (*   cbn. *)
 
-        cbn in VALID.
-        split.
-        + auto.
-        + apply get_fresh_provenance_fresh.
+      (*   split; [|split]. *)
+      (*   + reflexivity. *)
+      (*   + split. *)
+      (*     * intros sid' USED. *)
+      (*       apply VALID_SID in USED. *)
+      (*       auto. *)
+      (*     * intros pr' USED. *)
+      (*       assert (used_provenance (sid, pr) pr') as USED'. *)
+      (*       { cbn in USED. cbn. *)
+      (*         eapply provenance_lt_trans. *)
+      (*         eapply provenance_lt_next_provenance. *)
+      (*         eauto. *)
+      (*       } *)
+      (*       apply VALID_PR in USED'. *)
+      (*       eapply provenance_lt_trans; eauto. *)
+      (*       eapply provenance_lt_next_provenance. *)
+      (*   + split. *)
+      (*     * intros CONTRA. *)
+      (*       apply VALID_PR in CONTRA. *)
+      (*       pose proof provenance_lt_next_provenance pr as CONTRA2. *)
+      (*       pose proof provenance_lt_antisym _ _ CONTRA CONTRA2 as EQ. *)
+      (*       eapply next_provenance_neq; eauto. *)
+      (*     * eapply provenance_lt_next_provenance. *)
       - (* raise_oom *)
-        intros A ms oom_msg sid.
+        intros A ms oom_msg [sid pr].
         cbn.
         rewrite map_bind.
         setoid_rewrite Raise.raiseOOM_bind_itree.
@@ -492,13 +545,13 @@ Module Type MemoryExecInterpreter (LP : LLVMParams) (MP : MemoryParams LP) (MMEP
         intros EQ.
         pinversion EQ.
       - (* raise_ub *)
-        intros A ms oom_msg sid.
+        intros A ms oom_msg [sid pr].
         cbn.
         rewrite map_bind.
         setoid_rewrite Raise.raiseUB_bind_itree.
         reflexivity.
       - (* raise_error *)
-        intros A ms oom_msg sid.
+        intros A ms oom_msg [sid pr].
         cbn.
         rewrite map_bind.
         setoid_rewrite Raise.raise_bind_itree.
@@ -511,10 +564,10 @@ Module Type MemoryExecInterpreter (LP : LLVMParams) (MP : MemoryParams LP) (MMEP
 
     (** Handlers *)
     Definition E_trigger : E ~> MemStateFreshT (itree Effout) :=
-      fun R e sid m => r <- trigger e;; ret (m, (sid, r)).
+      fun R e sid pr m => r <- trigger e;; ret (m, (pr, (sid, r))).
 
     Definition F_trigger : F ~> MemStateFreshT (itree Effout) :=
-      fun R e sid m => r <- trigger e;; ret (m, (sid, r)).
+      fun R e sid pr m => r <- trigger e;; ret (m, (pr, (sid, r))).
 
     (* TODO: get rid of this silly hack. *)
     Definition my_handle_memory : MemoryE ~> MemStateFreshT (itree Effout) :=
@@ -538,7 +591,7 @@ Module Type MemoryExecInterpreter (LP : LLVMParams) (MP : MemoryParams LP) (MMEP
      *)
     Lemma interp_memory_correct :
       forall {T} t (ms : MemState) (sid : store_id) (pr : Provenance),
-        interp_memory_prop eq t sid ms (@interp_memory T t sid ms).
+        interp_memory_prop eq t sid pr ms (@interp_memory T t sid pr ms).
     Proof.
       intros T t ms sid pr.
       unfold interp_memory_prop.
